reorganize files

theories/MetaTheory/Conversion/TermConversion.v
@@ -1,8 +1,11 @@
 From Metaprog Require Import Prelude.
-From Metaprog.MetaTheory Require Export Confluence.
+From Metaprog.MetaTheory Require Export Reduction.Confluence.
 
-(** This module defines the conversion relation [conv] on [term]
-    and develops the equational theory of [conv]. *)
+(** This module defines the conversion relation [conv] on terms
+    and proves basic lemmas, notably:
+    - The Church-Rosser lemma.
+    - Congruence lemmas.
+    - Inversion lemmas (aka injectivity of constructors). *)
 
 (***********************************************************************)
 (** * Conversion relation on terms. *)
@@ -11,7 +14,8 @@ From Metaprog.MetaTheory Require Export Confluence.
 Reserved Notation "Γ ⊢ t ≡ u"
   (at level 50, no associativity, t at next level, u at next level).
 
-(** Conversion relation, defined as the smallest equivalence relation containing [red1]. *)
+(** Conversion relation on terms, defined as the smallest equivalence
+    relation containing [red1]. *)
 Inductive conv {s} Σ : term s -> term s -> Prop :=
 | conv_of_red1 t1 t2 : Σ ⊢ t1 ~> t2 -> Σ ⊢ t1 ≡ t2
 | conv_refl t : Σ ⊢ t ≡ t
@@ -39,20 +43,34 @@ intros H. induction H.
 - rewrite IHred. now apply conv_of_red1.
 Qed.
 
+#[export] Instance subrelation_red1_conv s Σ :
+  subrelation (@red1 s Σ) (@conv s Σ).
+Proof. intros t u H. now apply conv_of_red1. Qed.
+
+#[export] Instance subrelation_red1_conv_flip s Σ :
+  subrelation (Basics.flip (@red1 s Σ)) (@conv s Σ).
+Proof.
+intros t u H. unfold Basics.flip in H. symmetry.
+now apply conv_of_red1.
+Qed.
+
 #[export] Instance subrelation_red_conv s Σ :
   subrelation (@red s Σ) (@conv s Σ).
 Proof. intros t u H. now apply conv_of_red. Qed.
 
 #[export] Instance subrelation_red_conv_flip s Σ :
-  subrelation (@red s Σ) (Basics.flip (@conv s Σ)).
-Proof. intros t u H. unfold Basics.flip. symmetry. now apply conv_of_red. Qed.
+  subrelation (Basics.flip (@red s Σ)) (@conv s Σ).
+Proof.
+intros t u H. unfold Basics.flip in H. symmetry.
+now apply conv_of_red.
+Qed.
 
 (***********************************************************************)
-(** * Church-Rosser theorem. *)
+(** * Church-Rosser lemma. *)
 (***********************************************************************)
 
-(** The Church-Rosser theorem is a direct consequence of the confluence lemma.
-    We use Church-Rosser to prove inversion lemmas for [conv]. *)
+(** The Church-Rosser lemma is a direct consequence of the confluence lemma.
+    Using Church-Rosser, one can lift many lemmas from [red] to [conv]. *)
 Lemma church_rosser {s} Σ (t1 t2 : term s) :
   Σ ⊢ t1 ≡ t2 ->
   exists u, Σ ⊢ t1 ~~> u /\ Σ ⊢ t2 ~~> u.
@@ -183,120 +201,4 @@ Section InversionLemmas.
   Qed.
 
 End InversionLemmas.
-
-(***********************************************************************)
-(** * Conversion relation on substitutions. *)
-(***********************************************************************)
-
-(** Conversion on substitutions is just pointwise conversion.
-    We wrap the definition in a record to avoid setoid rewrite issues. *)
-Record sconv {s s'} (Σ : evar_map) (σ σ' : subst s s') : Prop := {
-  sconv_prop : forall i, Σ ⊢ sapply σ i ≡ sapply σ' i
-}.
-
-#[export] Instance sconv_Reflexive s s' Σ : Reflexive (@sconv s s' Σ).
-Proof. intros σ. constructor. reflexivity. Qed.
-
-#[export] Instance sconv_Symmetric s s' Σ : Symmetric (@sconv s s' Σ).
-Proof. intros σ σ' [Hσ]. constructor. intros i. now symmetry. Qed.
-
-#[export] Instance sconv_Transitive s s' Σ : Transitive (@sconv s s' Σ).
-Proof.
-intros σ1 σ2 σ3 [H1] [H2]. constructor. intros i. etransitivity ; eauto.
-Qed.
-
-#[export] Instance conv_sapply {s s'} Σ :
-  Proper (sconv Σ ==> eq ==> conv Σ) (@sapply s s').
-Proof. intros σ σ' [Hσ] i ? <-. apply Hσ. Qed.
-
-#[export] Instance sconv_of_sred {s s'} Σ :
-  subrelation (@sred s s' Σ) (@sconv s s' Σ).
-Proof. intros σ σ' Hσ. constructor. intros i. now rewrite Hσ. Qed.
-
-#[export] Instance sconv_of_sred_flip {s s'} Σ :
-  subrelation (Basics.flip (@sred s s' Σ)) (@sconv s s' Σ).
-Proof. intros σ σ' Hσ. constructor. intros i. now rewrite Hσ. Qed.
-
-(** Church Rosser lemma on substitutions.
-    This is a simple consequence of the Church Rosser lemma on terms. *)
-Lemma church_rosser_subst {s s' Σ} (σ σ' : subst s s') :
-  sconv Σ σ σ' ->
-  exists τ, sred Σ σ τ /\ sred Σ σ' τ.
-Proof.
-revert s' σ σ'. induction s.
-- intros s' σ σ' Hσ. exists (sren wk_idx). split ; constructor ; intros i ; depelim i.
-- intros s' σ σ' Hσ.
-  specialize (IHs s' (rscomp rshift σ) (rscomp rshift σ')).
-  forward IHs. { constructor. intros i. simpl_subst. now rewrite Hσ. }
-  destruct IHs as (τ & H1 & H2).
-  assert (exists t, Σ ⊢ sapply σ I0 ~~> t /\ Σ ⊢ sapply σ' I0 ~~> t) as (t & Ht1 & Ht2).
-  { apply church_rosser. now rewrite Hσ. }
-  exists (scons x t τ). split.
-  + constructor. intros i. depelim i ; simpl_subst.
-    * exact Ht1.
-    * destruct H1 as [H1]. specialize (H1 i). simpl_subst in H1. exact H1.
-  + constructor. intros i. depelim i ; simpl_subst.
-    * exact Ht2.
-    * destruct H2 as [H2]. specialize (H2 i). simpl_subst in H2. exact H2.
-Qed.
-
-(***********************************************************************)
-(** * Compatibility of conversion with substitution. *)
-(***********************************************************************)
-
-#[export] Instance conv_rename {s s' Σ} (ρ : ren s s') :
-  Proper (conv Σ ==> conv Σ) (rename ρ).
-Proof.
-intros t t' H. apply church_rosser in H. destruct H as (u & H1 & H2).
-now rewrite H1, H2.
-Qed.
-
-#[export] Instance conv_substitute {s s' Σ} :
-  Proper (sconv Σ ==> conv Σ ==> conv Σ) (@substitute s s').
-Proof.
-intros σ σ' Hσ t t' Ht.
-apply church_rosser in Ht. destruct Ht as (u & -> & ->).
-apply church_rosser_subst in Hσ. destruct Hσ as (? & -> & ->).
-reflexivity.
-Qed.
-
-#[export] Instance conv_scons {s s' x Σ} :
-  Proper (conv Σ ==> sconv Σ ==> sconv Σ) (@scons s s' x).
-Proof.
-intros t t' Ht σ σ' Hσ. constructor. intros i.
-apply church_rosser in Ht. destruct Ht as (? & -> & ->).
-apply church_rosser_subst in Hσ. destruct Hσ as (? & -> & ->).
-reflexivity.
-Qed.
-
-#[export] Instance conv_srcomp {s s' x Σ} :
-  Proper (sconv Σ ==> eq ==> sconv Σ) (@srcomp s s' x).
-Proof.
-intros σ σ' Hσ ρ ρ' <-. constructor. intros i.
-apply church_rosser_subst in Hσ. destruct Hσ as (? & -> & ->).
-reflexivity.
-Qed.
-
-#[export] Instance conv_rscomp {s s' x Σ} :
-  Proper (eq ==> sconv Σ ==> sconv Σ) (@rscomp s s' x).
-Proof.
-intros ρ ρ' <- σ σ' Hσ. constructor. intros i.
-apply church_rosser_subst in Hσ. destruct Hσ as (? & -> & ->).
-reflexivity.
-Qed.
-
-#[export] Instance conv_sup {s s' x Σ} :
-  Proper (sconv Σ ==> sconv Σ) (@sup s s' x).
-Proof.
-intros σ σ' Hσ. apply church_rosser_subst in Hσ.
-destruct Hσ as (? & -> & ->). reflexivity.
-Qed.
-
-#[export] Instance conv_scomp {s s' x Σ} :
-  Proper (sconv Σ ==> sconv Σ ==> sconv Σ) (@scomp s s' x).
-Proof.
-intros σ σ' Hσ τ τ' Hτ. apply church_rosser_subst in Hσ, Hτ.
-destruct Hσ as (? & -> & ->). destruct Hτ as (? & -> & ->).
-reflexivity.
-Qed.
 
