theories/MetaTheory/Reduction/TermReduction.v
@@ -3,10 +3,11 @@ From Metaprog.MetaTheory Require Export Relations Substitution EvarMap.
 
 (** This module defines:
     - The one-step strong reduction relation [red1] on terms.
-    - The strong reduction relation [red] on terms and its basic properties.
-
-    This module also defines reduction on related data-types such
-    as substitutions and context. *)
+    - The strong reduction relation [red] on terms.
+    And proves some basic properties, notably:
+    - Congruence lemmas.
+    - Inversion lemmas.
+*)
 
 (***********************************************************************)
 (** * One-step reduction relation [red1]. *)
@@ -254,7 +255,7 @@ Section CongruenceLemmas.
 End CongruenceLemmas.
 
 (***********************************************************************)
-(** * Inversion lemmas. *)
+(** * Inversion lemmas for [red]. *)
 (***********************************************************************)
 
 Section InversionLemmas.
@@ -309,128 +310,3 @@ Section InversionLemmas.
   Qed.
 
 End InversionLemmas.
-
-(***********************************************************************)
-(** * Reduction on substitutions. *)
-(***********************************************************************)
-
-(** Reduction on substitutions is just pointwise reduction.
-    We wrap the definition in a record because otherwise rewriting with
-    [H : sred Σ σ σ'] will sometimes fail due to setoid rewrite wanting to rewrite
-    [sapply σ i] into [sapply σ' i].  *)
-Record sred {s s'} Σ (σ σ' : subst s s') := {
-  sred_prop : forall i, Σ ⊢ sapply σ i ~~> sapply σ' i
-}.
-
-#[export] Instance sred_Reflexive s s' Σ : Reflexive (@sred s s' Σ).
-Proof. intros σ. constructor. reflexivity. Qed.
-
-#[export] Instance sred_Transitive s s' Σ : Transitive (@sred s s' Σ).
-Proof.
-intros σ1 σ2 σ3 [H1] [H2]. constructor. intros i. etransitivity ; eauto.
-Qed.
-
-#[export] Instance red_sapply {s s'} Σ :
-  Proper (sred Σ ==> eq ==> red Σ) (@sapply s s').
-Proof. intros σ σ' [Hσ] i ? <-. apply Hσ. Qed.
-
-(***********************************************************************)
-(** * Compatibility with renaming and substitution. *)
-(***********************************************************************)
-
-(** Compatibility of renaming with [red1]. *)
-#[export] Instance red1_rename {Σ s s'} (ρ : ren s s') :
-  Proper (red1 Σ ==> red1 Σ) (rename ρ).
-Proof.
-intros t t' H. induction H in s', ρ |- * ; simpl_subst.
-- cbn. apply red1_beta_alt. f_equal. now simpl_subst.
-- eapply red1_evar_expand. eassumption.
-- now apply red1_lam_l.
-- now apply red1_lam_r.
-- now apply red1_prod_l.
-- now apply red1_prod_r.
-- now apply red1_app_l.
-- apply red1_app_r, OnOne2_map. revert H. apply OnOne2_consequence. firstorder.
-Qed.
-
-(** Compatibility of renaming with [red]. *)
-#[export] Instance red_rename {Σ s s'} (ρ : ren s s') :
-  Proper (red Σ ==> red Σ) (rename ρ).
-Proof.
-intros t t' H. induction H.
-- reflexivity.
-- now rewrite IHred, H0.
-Qed.
-
-#[export] Instance red_scons {Σ s s' x} :
-  Proper (red Σ ==> sred Σ ==> sred Σ) (@scons s s' x).
-Proof.
-intros t t' Ht σ σ' Hσ. constructor. intros i. depelim i ; simpl_subst.
-- assumption.
-- now rewrite Hσ.
-Qed.
-
-#[export] Instance red_srcomp {Σ s s' s''} :
-  Proper (sred Σ ==> eq ==> sred Σ) (@srcomp s s' s'').
-Proof.
-intros σ σ' Hσ ρ ρ' <-. constructor. intros i. simpl_subst.
-now rewrite Hσ.
-Qed.
-
-#[export] Instance red_rscomp {Σ s s' s''} ρ :
-  Proper (sred Σ ==> sred Σ) (@rscomp s s' s'' ρ).
-Proof.
-intros σ σ' Hσ. constructor. intros i. simpl_subst.
-now rewrite Hσ.
-Qed.
-
-#[export] Instance red_sup {Σ s s' x} :
-  Proper (sred Σ ==> sred Σ) (@sup s s' x).
-Proof. intros σ σ' Hσ. unfold sup. now rewrite Hσ. Qed.
-
-(** Compatibility of substitution with [red1]. Note that a single reduction in
-    the substitution can cause several reductions in the result, so here we fix
-    the substitution [σ]. *)
-#[export] Instance red1_substitute_l {Σ s s'} (σ : subst s s') :
-  Proper (red1 Σ ==> red1 Σ) (substitute σ).
-Proof.
-intros t t' H. induction H in s', σ |- * ; simpl_subst.
-- cbn. apply red1_beta_alt. f_equal. now simpl_subst.
-- eapply red1_evar_expand. eassumption.
-- now apply red1_lam_l.
-- now apply red1_lam_r.
-- now apply red1_prod_l.
-- now apply red1_prod_r.
-- now apply red1_app_l.
-- apply red1_app_r, OnOne2_map. revert H. apply OnOne2_consequence. firstorder.
-Qed.
-
-(** Substitution lemma for [red]. *)
-#[export] Instance red_substitute {Σ s s'} :
-  Proper (sred Σ ==> red Σ ==> red Σ) (@substitute s s').
-Proof.
-intros σ σ' Hσ t t' H. transitivity (substitute σ' t).
-- clear t' H. induction t in s', σ, σ', Hσ |- * using term_ind' ; simpl_subst.
-  + reflexivity.
-  + now rewrite Hσ.
-  + f_equiv.
-    * now apply IHt1.
-    * apply IHt2. now f_equiv.
-  + f_equiv.
-    * now apply IHt1.
-    * apply IHt2. now f_equiv.
-  + f_equiv.
-    * now apply IHt.
-    * clear t IHt. induction H ; cbn ; constructor ; auto.
-  + reflexivity.
-- induction H.
-  + reflexivity.
-  + now rewrite IHred, H0.
-Qed.
-
-#[export] Instance red_scomp {Σ s s' s''} :
-  Proper (sred Σ ==> sred Σ ==> sred Σ) (@scomp s s' s'').
-Proof.
-intros σ σ' Hσ τ τ' Hτ. constructor. intros i. simpl_subst.
-now rewrite Hτ, Hσ.
-Qed.
