theories/MetaTheory/Conversion/ContextConversion.v
@@ -1,0 +1,70 @@
+From Metaprog Require Import Prelude.
+From Metaprog.MetaTheory Require Export Conversion.SubstConversion.
+
+(** This module defines the conversion relation [cconv] on contexts
+    and proves basic lemmas, notably the Church-Rosser lemma for contexts. *)
+
+(***********************************************************************)
+(** * Conversion relation on contexts. *)
+(***********************************************************************)
+
+(** [cconv Σ Γ Γ'] means that contexts [Γ] and [Γ'] are convertible
+    in evar-map [Σ]. *)
+Inductive cconv (Σ : evar_map) : forall {s}, context ∅ s -> context ∅ s -> Prop :=
+| cconv_nil : cconv Σ CNil CNil
+
+| cconv_cons {s} x (ty ty' : term s) Γ Γ' :
+    Σ ⊢ ty ≡ ty' ->
+    cconv Σ Γ Γ' ->
+    cconv Σ (CCons Γ x ty) (CCons Γ' x ty').
+
+Derive Signature for cconv.
+
+#[export] Instance cconv_Reflexive Σ s : Reflexive (@cconv Σ s).
+Proof.
+intros Γ. induction Γ ; constructor.
+- reflexivity.
+- assumption.
+Qed.
+
+#[export] Instance cconv_Symmetric Σ s : Symmetric (@cconv Σ s).
+Proof.
+intros Γ Γ' HΓ. induction HΓ ; constructor.
+- now symmetry.
+- assumption.
+Qed.
+
+#[export] Instance cconv_Transitive Σ s : Transitive (@cconv Σ s).
+Proof.
+intros Γ1 Γ2 Γ3 H1 H2. induction H1 ; depelim H2.
+- unfold eq_rect in H. cbn in H. depelim H. reflexivity.
+- unfold eq_rect in H3. cbn in H3. depelim H3. constructor.
+  + rewrite H. admit.
+  + apply IHcconv. admit.
+(* Equations issue: I need NoConfusionHom on [context]. *)
+Admitted.
+
+#[export] Instance cconv_of_cred1 Σ s : subrelation (@cred1 Σ s) (@cconv Σ s).
+Proof.
+intros Γ Γ' HΓ. induction HΓ ; constructor.
+- now rewrite H.
+- reflexivity.
+- reflexivity.
+- assumption.
+Qed.
+
+#[export] Instance cconv_of_cred Σ s : subrelation (@cred Σ s) (@cconv Σ s).
+Proof.
+intros Γ Γ' HΓ. induction HΓ ; constructor.
+- now rewrite H.
+- assumption.
+Qed.
+
+Lemma lookup_context_cconv {s Σ} (i : index s) Γ Γ' :
+  cconv Σ Γ Γ' ->
+  Σ ⊢ lookup_context i Γ ≡ lookup_context i Γ'.
+Proof.
+intros H. induction H ; depelim i ; simp lookup_context ; simpl_subst.
+- now rewrite H.
+- now rewrite IHcconv.
+Qed.
