theories/MetaTheory/Conversion/SubstConversion.v
@@ -1,0 +1,128 @@
+From Metaprog Require Import Prelude.
+From Metaprog.MetaTheory Require Export Conversion.TermConversion.
+
+(** This module defines the conversion relation [sconv] on substitutions
+    and proves basic lemmas, notably:
+    - The Church-Rosser lemma for substitutions.
+    - Compatibility of conversion with renaming and substitution. *)
+
+(***********************************************************************)
+(** * Conversion relation on substitutions. *)
+(***********************************************************************)
+
+(** Conversion on substitutions is just pointwise conversion.
+    We wrap the definition in a record to avoid setoid rewrite issues. *)
+Record sconv {s s'} (Σ : evar_map) (σ σ' : subst s s') : Prop := {
+  sconv_prop : forall i, Σ ⊢ sapply σ i ≡ sapply σ' i
+}.
+
+#[export] Instance sconv_Reflexive s s' Σ : Reflexive (@sconv s s' Σ).
+Proof. intros σ. constructor. reflexivity. Qed.
+
+#[export] Instance sconv_Symmetric s s' Σ : Symmetric (@sconv s s' Σ).
+Proof. intros σ σ' [Hσ]. constructor. intros i. now symmetry. Qed.
+
+#[export] Instance sconv_Transitive s s' Σ : Transitive (@sconv s s' Σ).
+Proof.
+intros σ1 σ2 σ3 [H1] [H2]. constructor. intros i. etransitivity ; eauto.
+Qed.
+
+#[export] Instance conv_sapply {s s'} Σ :
+  Proper (sconv Σ ==> eq ==> conv Σ) (@sapply s s').
+Proof. intros σ σ' [Hσ] i ? <-. apply Hσ. Qed.
+
+#[export] Instance sconv_of_sred {s s'} Σ :
+  subrelation (@sred s s' Σ) (@sconv s s' Σ).
+Proof. intros σ σ' Hσ. constructor. intros i. now rewrite Hσ. Qed.
+
+#[export] Instance sconv_of_sred_flip {s s'} Σ :
+  subrelation (Basics.flip (@sred s s' Σ)) (@sconv s s' Σ).
+Proof. intros σ σ' Hσ. constructor. intros i. now rewrite Hσ. Qed.
+
+(***********************************************************************)
+(** * Church-Rosser lemma. *)
+(***********************************************************************)
+
+(** Church-Rosser lemma on substitutions.
+    This is a simple consequence of the Church-Rosser lemma on terms. *)
+Lemma church_rosser_subst {s s' Σ} (σ σ' : subst s s') :
+  sconv Σ σ σ' ->
+  exists τ, sred Σ σ τ /\ sred Σ σ' τ.
+Proof.
+revert s' σ σ'. induction s.
+- intros s' σ σ' Hσ. exists (sren wk_idx). split ; constructor ; intros i ; depelim i.
+- intros s' σ σ' Hσ.
+  specialize (IHs s' (rscomp rshift σ) (rscomp rshift σ')).
+  forward IHs. { constructor. intros i. simpl_subst. now rewrite Hσ. }
+  destruct IHs as (τ & H1 & H2).
+  assert (exists t, Σ ⊢ sapply σ I0 ~~> t /\ Σ ⊢ sapply σ' I0 ~~> t) as (t & Ht1 & Ht2).
+  { apply church_rosser. now rewrite Hσ. }
+  exists (scons x t τ). split.
+  + constructor. intros i. depelim i ; simpl_subst.
+    * exact Ht1.
+    * destruct H1 as [H1]. specialize (H1 i). simpl_subst in H1. exact H1.
+  + constructor. intros i. depelim i ; simpl_subst.
+    * exact Ht2.
+    * destruct H2 as [H2]. specialize (H2 i). simpl_subst in H2. exact H2.
+Qed.
+
+(***********************************************************************)
+(** * Compatibility of conversion with renaming and substitution. *)
+(***********************************************************************)
+
+#[export] Instance conv_rename {s s' Σ} (ρ : ren s s') :
+  Proper (conv Σ ==> conv Σ) (rename ρ).
+Proof.
+intros t t' H. apply church_rosser in H. destruct H as (u & H1 & H2).
+now rewrite H1, H2.
+Qed.
+
+#[export] Instance conv_substitute {s s' Σ} :
+  Proper (sconv Σ ==> conv Σ ==> conv Σ) (@substitute s s').
+Proof.
+intros σ σ' Hσ t t' Ht.
+apply church_rosser in Ht. destruct Ht as (u & -> & ->).
+apply church_rosser_subst in Hσ. destruct Hσ as (? & -> & ->).
+reflexivity.
+Qed.
+
+#[export] Instance conv_scons {s s' x Σ} :
+  Proper (conv Σ ==> sconv Σ ==> sconv Σ) (@scons s s' x).
+Proof.
+intros t t' Ht σ σ' Hσ. constructor. intros i.
+apply church_rosser in Ht. destruct Ht as (? & -> & ->).
+apply church_rosser_subst in Hσ. destruct Hσ as (? & -> & ->).
+reflexivity.
+Qed.
+
+#[export] Instance conv_srcomp {s s' x Σ} :
+  Proper (sconv Σ ==> eq ==> sconv Σ) (@srcomp s s' x).
+Proof.
+intros σ σ' Hσ ρ ρ' <-. constructor. intros i.
+apply church_rosser_subst in Hσ. destruct Hσ as (? & -> & ->).
+reflexivity.
+Qed.
+
+#[export] Instance conv_rscomp {s s' x Σ} :
+  Proper (eq ==> sconv Σ ==> sconv Σ) (@rscomp s s' x).
+Proof.
+intros ρ ρ' <- σ σ' Hσ. constructor. intros i.
+apply church_rosser_subst in Hσ. destruct Hσ as (? & -> & ->).
+reflexivity.
+Qed.
+
+#[export] Instance conv_sup {s s' x Σ} :
+  Proper (sconv Σ ==> sconv Σ) (@sup s s' x).
+Proof.
+intros σ σ' Hσ. apply church_rosser_subst in Hσ.
+destruct Hσ as (? & -> & ->). reflexivity.
+Qed.
+
+#[export] Instance conv_scomp {s s' x Σ} :
+  Proper (sconv Σ ==> sconv Σ ==> sconv Σ) (@scomp s s' x).
+Proof.
+intros σ σ' Hσ τ τ' Hτ. apply church_rosser_subst in Hσ, Hτ.
+destruct Hσ as (? & -> & ->). destruct Hτ as (? & -> & ->).
+reflexivity.
+Qed.
+
