theories/MetaTheory/Reduction/ContextReduction.v
@@ -1,0 +1,90 @@
+From Metaprog Require Import Prelude.
+From Metaprog Require Export Data.Context MetaTheory.Reduction.SubstReduction.
+
+(** This module defines:
+    - One-step reduction of contexts [cred1].
+    - Multi-step reduction of contexts [cred].
+    And proves basic properties.
+*)
+
+(***********************************************************************)
+(** * One-step reduction of contexts. *)
+(***********************************************************************)
+
+(** [cred1 Σ Γ Γ'] means that context [Γ] reduces to context [Γ'] in
+    exactly one reduction step. *)
+Inductive cred1 (Σ : evar_map) : forall {s}, context ∅ s -> context ∅ s -> Prop :=
+| cred1_head {s} Γ x (ty ty' : term s) :
+    Σ ⊢ ty ~> ty' ->
+    cred1 Σ (CCons Γ x ty) (CCons Γ x ty')
+
+| cred1_tail {s} Γ Γ' x (ty : term s) :
+    cred1 Σ Γ Γ' ->
+    cred1 Σ (CCons Γ x ty) (CCons Γ' x ty).
+
+Derive Signature for cred1.
+
+Lemma lookup_context_cred1 {s Σ} (i : index s) Γ Γ' :
+  cred1 Σ Γ Γ' ->
+  Σ ⊢ lookup_context i Γ ~> lookup_context i Γ' \/
+  lookup_context i Γ = lookup_context i Γ'.
+Proof.
+intros Hred. induction Hred ; depelim i ; simp lookup_context ; simpl_subst.
+- left. now apply red1_rename.
+- now right.
+- now right.
+- destruct (IHHred i) as [H1 | H2].
+  + left. apply red1_rename. apply H1.
+  + right. now rewrite H2.
+Qed.
+
+(***********************************************************************)
+(** * Multi-step reduction of contexts. *)
+(***********************************************************************)
+
+(** [cred Σ Γ Γ'] means that context [Γ] reduces to context [Γ'] in
+    zero or more reduction step. *)
+Inductive cred (Σ : evar_map) : forall {s}, context ∅ s -> context ∅ s -> Prop :=
+| cred_nil : cred Σ CNil CNil
+
+| cred_cons {s} x (ty ty' : term s) Γ Γ' :
+    Σ ⊢ ty ~~> ty' ->
+    cred Σ Γ Γ' ->
+    cred Σ (CCons Γ x ty) (CCons Γ' x ty').
+
+Derive Signature for cred.
+
+#[export] Instance cred_Reflexive Σ s : Reflexive (@cred Σ s).
+Proof.
+intros Γ. induction Γ ; constructor.
+- reflexivity.
+- assumption.
+Qed.
+
+#[export] Instance cred_Transitive Σ s : Transitive (@cred Σ s).
+Proof.
+intros Γ1 Γ2 Γ3 H1 H2. induction H1 ; depelim H2.
+- unfold eq_rect in H. cbn in H. depelim H. reflexivity.
+- unfold eq_rect in H3. cbn in H3. depelim H3. constructor.
+  + rewrite H. admit.
+  + apply IHcred. admit.
+(* Equations issue: I need NoConfusionHom on [context]. *)
+Admitted.
+
+#[export] Instance cred_of_cred1 Σ s : subrelation (@cred1 Σ s) (@cred Σ s).
+Proof.
+intros Γ Γ' HΓ. induction HΓ ; constructor.
+- now rewrite H.
+- reflexivity.
+- reflexivity.
+- assumption.
+Qed.
+
+Lemma lookup_context_cred {s Σ} (i : index s) Γ Γ' :
+  cred Σ Γ Γ' ->
+  Σ ⊢ lookup_context i Γ ~~> lookup_context i Γ'.
+Proof.
+intros H. induction H ; depelim i ; simp lookup_context ; simpl_subst.
+- now rewrite H.
+- now rewrite IHcred.
+Qed.
