theories/MetaTheory/Typing/EvarMapTyping.v
@@ -1,0 +1,41 @@
+From Metaprog Require Import Prelude.
+From Metaprog Require Export MetaTheory.Typing.TermTyping.
+
+(** This module defines a notion of typing for evar-maps. *)
+
+(***********************************************************************)
+(** * Typing evar-maps. *)
+(***********************************************************************)
+
+(** [typing_evar_entry Σ e] asserts that the evar-entry [e] is well-typed
+    in evar-map [Σ]. *)
+Inductive typing_evar_entry (Σ : evar_map) : evar_entry -> Prop :=
+
+(** An undefined evar entry is well-typed if the type if well-typed. *)
+| typing_evar_undefined ty :
+    Σ ;; CNil ⊢ ty : TType ->
+    typing_evar_entry Σ (mk_evar_entry ty None)
+
+(** A defined evar entry is well-typed if the type is well-typed
+    and the definition has the correct type. *)
+| typing_evar_defined ty def :
+    Σ ;; CNil ⊢ ty : TType ->
+    Σ ;; CNil ⊢ def : ty ->
+    typing_evar_entry Σ (mk_evar_entry ty (Some def)).
+
+Derive Signature for typing_evar_entry.
+
+(** [typing_evar_map Σ] means that the evar-map [Σ] is well-typed.
+    We do _not_ check that the evar-map is acyclic:
+    this would likely be very annoying to do. *)
+Definition typing_evar_map (Σ : evar_map) :=
+  forall ev entry, Σ ev = Some entry -> typing_evar_entry Σ entry.
+
+(***********************************************************************)
+(** * Properties of evar-map typing. *)
+(***********************************************************************)
+
+Lemma typing_evar_type Σ entry :
+  typing_evar_entry Σ entry ->
+  Σ ;; CNil ⊢ entry.(evar_type) : TType.
+Proof. intros H. destruct H ; cbn ; assumption. Qed.
