theories/MetaTheory/Typing/TermTyping.v
@@ -1,0 +1,330 @@
+From Metaprog Require Import Prelude.
+From Metaprog Require Export Data.Context MetaTheory.Conversion.ContextConversion.
+
+(** This module defines the typing relations on terms and contexts
+    and their basic properties, notably inversion lemmas.
+*)
+
+(***********************************************************************)
+(** * Lifting a typing-like relation on a context. *)
+(***********************************************************************)
+
+Section All_context.
+  Context (P : forall s, context ∅ s -> term s -> term s -> Prop).
+
+  (** [All_context P Γ] lifts the relation [P] over the context [Γ]. *)
+  Inductive All_context : forall {s}, context ∅ s -> Prop :=
+  | All_context_nil : All_context CNil
+
+  | All_context_cons {s} (Γ : context ∅ s) x ty :
+      All_context Γ ->
+      P s Γ ty TType ->
+      All_context (CCons Γ x ty).
+End All_context.
+
+Derive Signature for All_context.
+
+Lemma All_context_consequence (P Q : forall s, context ∅ s -> term s -> term s -> Prop) :
+  (forall s Γ t T, P s Γ t T -> Q s Γ t T) ->
+  forall s (Γ : context ∅ s), All_context P Γ -> All_context Q Γ.
+Proof.
+intros Himpl s Γ H. induction H ; econstructor ; eauto.
+Qed.
+
+Lemma All_context_and {P Q : forall s, context ∅ s -> term s -> term s -> Prop} {s} {Γ : context ∅ s} :
+  All_context (fun s Γ t T => P s Γ t T /\ Q s Γ t T) Γ ->
+  (All_context P Γ /\ All_context Q Γ).
+Proof.
+induction Γ.
+- constructor ; constructor.
+- intros H. depelim H. apply IHΓ in H. split ; now constructor.
+Qed.
+
+(***********************************************************************)
+(** * Lifting a typing-like relation on a spine of arguments. *)
+(***********************************************************************)
+
+Section All_spine.
+  Context {s : scope} (Σ : evar_map).
+  Context (P : term s -> term s -> Prop).
+
+  (** [All_spine Σ P] lifts the relation [P] to a spine of arguments.
+      If [P] is [typing Σ Γ], then [All_spine Σ P f_ty args T] means
+      that appling a function of type [f_ty] to the list of arguments
+      [args] yields a term of type [T]. *)
+  Inductive All_spine : term s -> list (term s) -> term s -> Prop :=
+  | All_spine_nil f_ty : All_spine f_ty [] f_ty
+
+  | All_spine_cons f_ty x a b arg args T :
+      P (TProd x a b) TType ->
+      Σ ⊢ f_ty ≡ TProd x a b ->
+      P arg a ->
+      All_spine (b[x := arg]) args T ->
+      All_spine f_ty (arg :: args) T.
+End All_spine.
+
+Derive Signature for All_spine.
+
+Lemma All_spine_consequence {s Σ} {P Q : term s -> term s -> Prop} :
+  (forall t T, P t T -> Q t T) ->
+  forall f_ty args (T : term s),
+    All_spine Σ P f_ty args T ->
+    All_spine Σ Q f_ty args T.
+Proof.
+intros Himpl f_ty args T H. induction H ; econstructor ; eauto.
+Qed.
+
+(** In [All_spine Σ P f_ty args T] we can change the function type [f_ty]
+    to a convertible one, as long as we are willing to accept that the return
+    type [T] also changes to a convertible one. *)
+Lemma All_spine_conv_func_type {s} Σ P f_ty f_ty' args (T : term s) :
+  All_spine Σ P f_ty args T ->
+  Σ ⊢ f_ty ≡ f_ty' ->
+  exists T',
+    All_spine Σ P f_ty' args T' /\
+    Σ ⊢ T ≡ T'.
+Proof.
+intros Hspine Hconv. induction Hspine in f_ty', Hconv |- *.
+- exists f_ty'. split ; [constructor | assumption].
+- specialize (IHHspine (b[x := arg])). forward IHHspine by reflexivity.
+  destruct IHHspine as (T' & Hspine' & HconvT).
+  exists T'. split ; auto. econstructor ; eauto. now rewrite <-Hconv.
+Qed.
+
+(***********************************************************************)
+(** * Typing relation on terms. *)
+(***********************************************************************)
+
+Unset Elimination Schemes.
+
+Reserved Notation "Σ ;; Γ ⊢ t : T"
+  (at level 50, no associativity, Γ, t, T at next level).
+
+Reserved Notation "'ctyping' Σ Γ"
+  (at level 9, no associativity, Σ, Γ at next level).
+
+Reserved Notation "'spine_typing' Σ Γ f_ty args T"
+  (at level 9, Σ, Γ, f_ty, args, T at next level).
+
+(** [Σ ;; Γ ⊢ t : T] means that [t] has type [T] under context [Γ] in evar-map [Σ].
+
+    [ctyping Σ Γ] means that context [Γ] only contains well-typed types.
+    [ctyping] is a notation on top of [All_context].
+
+    [spine_typing Σ Γ f_ty args T] means that applying a function of type [f_ty]
+    to arguments [args] results in a term of type [T].
+    [spine_typing] is a notation on top of [All_spine].
+*)
+Inductive typing (Σ : evar_map) {s} (Γ : context ∅ s) : term s -> term s -> Prop :=
+
+| typing_type :
+    ctyping Σ Γ ->
+    Σ ;; Γ ⊢ TType : TType
+
+| typing_var i ty :
+    ctyping Σ Γ ->
+    lookup_context i Γ = ty ->
+    Σ ;; Γ ⊢ TVar i : ty
+
+| typing_lam x ty body body_ty :
+    Σ ;; Γ ⊢ ty : TType ->
+    Σ ;; CCons Γ x ty ⊢ body : body_ty ->
+    Σ ;; Γ ⊢ TLam x ty body : TProd x ty body_ty
+
+| typing_prod x a b :
+    Σ ;; Γ ⊢ a : TType ->
+    Σ ;; CCons Γ x a ⊢ b : TType ->
+    Σ ;; Γ ⊢ TProd x a b : TType
+
+| typing_app f f_ty args T :
+    Σ ;; Γ ⊢ f : f_ty ->
+    spine_typing Σ Γ f_ty args T ->
+    Σ ;; Γ ⊢ TApp f args : T
+
+| typing_evar ev entry :
+    ctyping Σ Γ ->
+    Σ ev = Some entry ->
+    Σ ;; Γ ⊢ TEvar ev : wk entry.(evar_type)
+
+| typing_conv_type t A B :
+    Σ ;; Γ ⊢ t : A ->
+    Σ ⊢ A ≡ B ->
+    Σ ;; Γ ⊢ B : TType ->
+    Σ ;; Γ ⊢ t : B
+
+where "Σ ;; Γ ⊢ t : T" := (typing Σ Γ t T)
+   and "'ctyping' Σ Γ" := (All_context (@typing Σ) Γ)
+   and "'spine_typing' Σ Γ f_ty args T" := (All_spine Σ (typing Σ Γ) f_ty args T).
+
+Set Elimination Schemes.
+
+Derive Signature for typing.
+
+(***********************************************************************)
+(** * Induction principle for [typing]. *)
+(***********************************************************************)
+
+(** Induction principle for [typing]. *)
+Lemma typing_ind
+  (P : evar_map -> forall s, context ∅ s -> term s -> term s -> Prop)
+  (Htype : forall s Σ Γ,
+    All_context (fun s' Γ' t T => Σ ;; Γ' ⊢ t : T /\ P Σ s' Γ' t T) Γ ->
+    P Σ s Γ TType TType)
+  (Hvar : forall s Σ Γ i ty,
+    All_context (fun s' Γ' t T => Σ ;; Γ' ⊢ t : T /\ P Σ s' Γ' t T) Γ ->
+    lookup_context i Γ = ty ->
+    P Σ s Γ (TVar i) ty)
+  (Hlam : forall s Σ Γ x ty body body_ty,
+    Σ ;; Γ ⊢ ty : TType -> P Σ s Γ ty TType ->
+    Σ ;; CCons Γ x ty ⊢ body : body_ty -> P Σ (s ▷ x) (CCons Γ x ty) body body_ty ->
+    P Σ s Γ (TLam x ty body) (TProd x ty body_ty))
+  (Hprod : forall s Σ Γ x a b,
+    Σ ;; Γ ⊢ a : TType -> P Σ s Γ a TType ->
+    Σ ;; CCons Γ x a ⊢ b : TType -> P Σ (s ▷ x) (CCons Γ x a) b TType ->
+    P Σ s Γ (TProd x a b) TType)
+  (Happ : forall s Σ Γ f f_ty args T,
+    Σ ;; Γ ⊢ f : f_ty -> P Σ s Γ f f_ty ->
+    All_spine Σ (fun t T => Σ ;; Γ ⊢ t : T /\ P Σ s Γ t T) f_ty args T ->
+    P Σ s Γ (TApp f args) T)
+  (Hevar : forall s Σ Γ ev entry,
+    All_context (fun s' Γ' t T => Σ ;; Γ' ⊢ t : T /\ P Σ s' Γ' t T) Γ ->
+    Σ ev = Some entry ->
+    P Σ s Γ (TEvar ev) (wk entry.(evar_type)))
+  (Hconv_type : forall s Σ Γ t A B,
+    Σ ;; Γ ⊢ t : A -> P Σ s Γ t A ->
+    Σ ⊢ A ≡ B ->
+    Σ ;; Γ ⊢ B : TType -> P Σ s Γ B TType ->
+    P Σ s Γ t B) :
+  forall Σ s Γ t T, Σ ;; Γ ⊢ t : T -> P Σ s Γ t T.
+Proof.
+fix IH 6. intros Σ s Γ t T H. depelim H.
+- apply Htype. revert s Γ H. fix IHctx 3. intros s Γ H. destruct H ; constructor.
+  + apply IHctx. assumption.
+  + split ; auto.
+- apply Hvar ; auto. subst. clear i. revert s Γ H. fix IHctx 3. intros s Γ H. destruct H ; constructor.
+  + apply IHctx. assumption.
+  + split ; auto.
+- apply Hlam ; auto.
+- apply Hprod ; auto.
+- apply Happ with f_ty ; auto. clear f H. revert f_ty args T H0.
+  fix IHspine 4. intros f_ty args T H0. destruct H0.
+  + constructor.
+  + econstructor ; eauto.
+- apply Hevar ; auto. revert s Γ H. fix IHctx 3. intros s Γ H. destruct H ; constructor.
+  + apply IHctx. assumption.
+  + split ; auto.
+- eapply Hconv_type ; eauto.
+Qed.
+
+(** In any typing derivation [Σ ;; Γ ⊢ t : T] the context [Γ] is well-typed. *)
+Lemma typing_context_validity {s} Σ Γ (t T : term s) :
+  Σ ;; Γ ⊢ t : T ->
+  ctyping Σ Γ.
+Proof.
+intros H. induction H ; auto.
+all: revert H ; now apply All_context_consequence.
+Qed.
+
+(***********************************************************************)
+(** * Inverting typing derivations. *)
+(***********************************************************************)
+
+(** Inverting typing derivations is not completely trivial:
+    indeed typing looks syntax directed at first glance, but in fact
+    it is _not_ because of the rule [typing_conv_type]. *)
+
+Lemma typing_type_inv {s} Σ Γ T :
+  Σ ;; Γ ⊢ TType : T ->
+  Σ ⊢ T ≡ @TType s.
+Proof.
+intros H. depind H.
+- reflexivity.
+- now rewrite <-H0.
+Qed.
+
+Lemma typing_var_inv {s} Σ Γ (i : index s) T :
+  Σ ;; Γ ⊢ TVar i : T ->
+  Σ ⊢ T ≡ lookup_context i Γ.
+Proof.
+intros H. depind H.
+- now subst.
+- now rewrite <-H0.
+Qed.
+
+Lemma typing_lam_inv_aux {s x} Σ Γ (t : term s) T :
+  Σ ;; Γ ⊢ t : T ->
+  forall ty body, t = TLam x ty body ->
+  exists body_ty,
+    Σ ⊢ T ≡ TProd x ty body_ty /\
+    Σ ;; Γ ⊢ ty : TType /\
+    Σ ;; CCons Γ x ty ⊢ body : body_ty.
+Proof.
+intros H. induction H ; intros ty' body' Ht ; depelim Ht.
+- exists body_ty. now split3.
+- destruct (IHtyping1 ty' body' eq_refl) as (body_ty' & HA & Hty & Hbody).
+  exists body_ty'. split3 ; auto. now rewrite <-H0.
+Qed.
+
+Lemma typing_lam_inv {s x} Σ Γ (ty : term s) body T :
+  Σ ;; Γ ⊢ TLam x ty body : T ->
+  exists body_ty,
+    Σ ⊢ T ≡ TProd x ty body_ty /\
+    Σ ;; Γ ⊢ ty : TType /\
+    Σ ;; CCons Γ x ty ⊢ body : body_ty.
+Proof. intros H. eapply typing_lam_inv_aux ; eauto. Qed.
+
+Lemma typing_prod_inv_aux {s x} Σ Γ (t : term s) T :
+  Σ ;; Γ ⊢ t : T ->
+  forall a b, t = TProd x a b ->
+    Σ ⊢ T ≡ TType /\
+    Σ ;; Γ ⊢ a : TType /\
+    Σ ;; CCons Γ x a ⊢ b : TType.
+Proof.
+intros H. induction H ; intros a' b' Ht ; depelim Ht.
+- now split3.
+- destruct (IHtyping1 a' b' eq_refl) as (HA & Ha & Hb).
+  split3 ; auto. now rewrite <-H0.
+Qed.
+
+Lemma typing_prod_inv {s x} Σ Γ (a : term s) b T :
+  Σ ;; Γ ⊢ TProd x a b : T ->
+  Σ ⊢ T ≡ TType /\ Σ ;; Γ ⊢ a : TType /\ Σ ;; CCons Γ x a ⊢ b : TType.
+Proof. intros H. eapply typing_prod_inv_aux ; eauto. Qed.
+
+Lemma typing_app_inv_aux {s} Σ Γ t (T : term s) :
+  Σ ;; Γ ⊢ t : T ->
+  forall f args, t = TApp f args ->
+  exists f_ty T',
+    Σ ;; Γ ⊢ f : f_ty /\
+    All_spine Σ (typing Σ Γ) f_ty args T' /\
+    Σ ⊢ T' ≡ T.
+Proof.
+intros H. induction H ; intros f' args' Ht ; depelim Ht.
+- assert (H1 : All_spine Σ (typing Σ Γ) f_ty args T).
+  { revert H0. apply All_spine_consequence. firstorder. }
+  clear IHtyping H0. exists f_ty, T. now split3.
+- destruct (IHtyping1 f' args' eq_refl) as (f_ty' & T' & Hf & H3).
+  exists f_ty', T'. split3 ; auto.
+  + apply H3.
+  + rewrite <-H0. apply H3.
+Qed.
+
+Lemma typing_app_inv {s} Σ Γ f args (T : term s) :
+  Σ ;; Γ ⊢ TApp f args : T ->
+  exists f_ty T',
+    Σ ;; Γ ⊢ f : f_ty /\
+    All_spine Σ (typing Σ Γ) f_ty args T' /\
+    Σ ⊢ T' ≡ T.
+Proof. intros H. eapply typing_app_inv_aux ; eauto. Qed.
+
+Lemma typing_evar_inv {s} Σ Γ ev (T : term s) :
+  Σ ;; Γ ⊢ TEvar ev : T ->
+  exists entry,
+    Σ ev = Some entry /\
+    Σ ⊢ T ≡ wk entry.(evar_type).
+Proof.
+intros H. depind H.
+- exists entry. now split.
+- destruct IHtyping1 as (entry & H2 & H3). exists entry.
+  split ; auto. now rewrite <-H0.
+Qed.
