theories/MetaTheory/Typing/Validity.v
@@ -1,0 +1,89 @@
+From Metaprog Require Import Prelude.
+From Metaprog Require Export MetaTheory.Typing.SubstTyping.
+
+(** This module proves two basic lemmas about the typing relation:
+    - The validity lemma: in any typing derivation [Σ ;; Γ ⊢ t : T],
+      [T] is itself well-typed.
+    - Uniqueness of types (up to conversion).
+*)
+
+Lemma typing_lookup_context {s} Σ (Γ : context ∅ s) i :
+  ctyping Σ Γ ->
+  Σ ;; Γ ⊢ lookup_context i Γ : TType.
+Proof.
+intros H. induction H.
+- depelim i.
+- depelim i ; simp lookup_context ; simpl_subst.
+  + change TType with (rename (@rshift s x) TType).
+    eapply typing_rename ; eauto. apply typing_rshift. constructor ; auto.
+  + change TType with (rename (@rshift s x) TType).
+    eapply typing_rename ; eauto. apply typing_rshift. constructor ; auto.
+Qed.
+
+(***********************************************************************)
+(** * Validity lemma. *)
+(***********************************************************************)
+
+(** The validity lemma for typing states that in any typing derivation,
+    the type is well-typed. *)
+Lemma typing_validity {s} Σ Γ (t T : term s) :
+  typing_evar_map Σ ->
+  Σ ;; Γ ⊢ t : T ->
+  Σ ;; Γ ⊢ T : TType.
+Proof.
+intros HΣ H. induction H.
+- constructor. revert H. apply All_context_consequence. firstorder.
+- subst. apply typing_lookup_context. revert H.
+  apply All_context_consequence. firstorder.
+- constructor ; auto.
+- constructor. eapply typing_context_validity ; eauto.
+- specialize (IHtyping HΣ).
+  assert (H1 : All_spine Σ (fun t T => Σ ;; Γ ⊢ t : T /\ Σ ;; Γ ⊢ T : TType) f_ty args T).
+  { revert H0. apply All_spine_consequence. firstorder. }
+  clear H H0. induction H1.
+  + assumption.
+  + apply IHAll_spine. destruct H as (H & _). apply typing_prod_inv in H.
+    destruct H as (_ & Ha & Hb). change TType with (TType[x := arg]).
+    eapply typing_substitute ; eauto. apply typing_scons.
+    * assumption.
+    * simpl_subst. apply H1.
+    * apply typing_sid. eapply typing_context_validity ; eauto.
+- simpl_subst. change TType with (@rename ∅ s wk_idx TType). eapply typing_rename.
+  + apply typing_evar_type. now apply (HΣ ev).
+  + split3.
+    * constructor.
+    * revert H. apply All_context_consequence. firstorder.
+    * intros i. depelim i.
+- assumption.
+Qed.
+
+(***********************************************************************)
+(** * Uniqueness of types. *)
+(***********************************************************************)
+
+(** Types are unique (up to convertibility). This lemma will no longer be true
+    once we add subtyping (with universes). *)
+Lemma typing_unique_type {s} Σ Γ (t A A' : term s) :
+  Σ ;; Γ ⊢ t : A ->
+  Σ ;; Γ ⊢ t : A' ->
+  Σ ⊢ A ≡ A'.
+Proof.
+intros HA. revert A'. induction HA ; intros A' HA'.
+- apply typing_type_inv in HA'. now symmetry.
+- subst. apply typing_var_inv in HA'. now symmetry.
+- apply typing_lam_inv in HA'. destruct HA' as (body_ty' & HA' & Hty & Hbody).
+  rewrite HA'. f_equiv. apply IHHA2. assumption.
+- apply typing_prod_inv in HA'. now symmetry.
+- apply typing_app_inv in HA'. destruct HA' as (f_ty' & T' & Hf' & Hspine & H1).
+  apply IHHA in Hf'. rewrite <-H1.
+  assert (H2 : All_spine Σ (typing Σ Γ) f_ty args T).
+  { revert H. apply All_spine_consequence. firstorder. }
+  clear A' H1 IHHA H HA. induction args in f_ty, f_ty', Hf', Hspine, H2 |- *.
+  + depelim Hspine ; depelim H2. assumption.
+  + depelim Hspine ; depelim H2. eapply IHargs ; [| eassumption.. ].
+    assert (x0 = x) as ->. { destruct x0 ; destruct x ; reflexivity. }
+    f_equiv. rewrite H0, H3 in Hf'. now apply conv_prod_inv in Hf'.
+- apply typing_evar_inv in HA'. destruct HA' as (entry' & Hentry & HA').
+  rewrite H0 in Hentry. depelim Hentry. now symmetry.
+- rewrite <-H. now apply IHHA1.
+Qed.
